qstar/src/QStar.Steel.Util.fst
@@ -1,0 +1,12 @@
+module QStar.Steel.Util
+open Steel.ST.Util
+#push-options "--ide_id_info_off"
+
+[@@warn_on_use "uses an axiom"]
+noextract
+val admit__ (#a:Type)
+            (#p:pre_t)
+            (#q:a -> vprop)
+            (_:unit)
+  : STF a p q True (fun _ -> False)
+
