qstar/src/QStarRef.fsti
@@ -1,0 +1,148 @@
+module QStarRef
+open Steel.ST.Util
+open QStar.Steel.Util
+open QVec
+open QStarHeap
+module M = Matrix
+#push-options "--ide_id_info_off"
+
+val pts_to (qs:qbits) ([@@@smt_fallback]state:qvec qs) : vprop
+
+val apply_gate (#qs:qbits) (#state:qvec qs) (gate:qvec qs -> qvec qs)
+  : STT unit
+    (pts_to qs state)
+    (fun _ -> pts_to qs (gate state))
+
+val share (#o:_) (qs:qbits) (qs':qbits{ disjoint_qbits qs qs'}) (#state:qvec qs) (#state':qvec qs')
+  : STGhostT unit o
+    (pts_to (qs `OrdSet.union` qs')
+            (state `tensor` state'))
+    (fun _ -> pts_to qs state `star` pts_to qs' state')
+
+val gather (#o:_) (qs:qbits) (qs':qbits) (#state:qvec qs) (#state':qvec qs')
+  : STGhostT (_:unit{disjoint_qbits qs qs'}) o
+    (pts_to qs state `star` pts_to qs' state')
+    (fun _ -> pts_to (qs `OrdSet.union` qs') (state `tensor` state'))
+
+
+let single (q:qbit) : qbits = OrdSet.singleton q
+let singleton q (b:bool) : qvec (single q) = M.create 2 1 (if b then Complex.c0 else Complex.c1)
+
+val project (q:qbit)
+            (qs:qbits {q `OrdSet.mem` qs })
+            (b:bool)
+            (s:qvec qs)
+  : option (qvec (qs `OrdSet.minus` single q))
+
+let disc (q:qbit)
+         (qs:qbits {q `OrdSet.mem` qs })
+         (b:bool)
+         (s:qvec qs { Some? (project q qs b s) })
+  : qvec (qs `OrdSet.minus` single q)
+  = Some?.v (project q qs b s)
+
+val measure (q:qbit)
+            (qs:qbits { q `OrdSet.mem` qs })
+            (state:qvec qs)
+  : STT (b:bool { Some? (project q qs b state) })
+    (pts_to qs state)
+    (fun b -> pts_to (single q) (singleton q b) `star`
+           pts_to (qs `OrdSet.minus` (single q)) (disc q qs b state))
+
+val alloc (_:unit)
+  : STT qbit emp (fun q -> pts_to (single q) (singleton q false))
+
+val discard (q:qbit) (qstate:qvec (single q))
+  : STT unit (pts_to (single q) qstate) (fun _ -> emp)
+
+val hadamard (q:qbit) : qvec (single q) -> qvec (single q)
+
+let self_adjoint (#qs:qbits) (gate: qvec qs -> qvec qs) =
+  forall (s:qvec qs). gate (gate s) == s
+
+val hadamard_self_adjoint (q:qbit)
+  : Lemma (ensures self_adjoint (hadamard q))
+          
+  
+let test1 (_:unit)
+  : STT unit emp (fun _ -> emp)
+  = //allocate a qbit q in |0>
+    let q = alloc () in
+    //apply H to it twice
+    apply_gate (hadamard q);
+    apply_gate (hadamard q);
+    //now we know q is in state H (H |0>)
+    assert_ (pts_to (single q) (hadamard q (hadamard q (singleton q false))));
+    //call the lemma below, and prove that q is actually back to |0>
+    hadamard_self_adjoint q;
+    rewrite (pts_to (single q) _)
+            (pts_to (single q) (singleton q false)); //use hadamard_self_adjoint to prove 
+                                                     //that q is back to its initial state
+    //discard it
+    discard q _
+
+// same as test1, but now with some other qbit around
+let test2 (_:unit)
+  : STT qbit emp (fun q1 -> pts_to (single q1) (hadamard _ (singleton _ false)))
+  = //allocate a qbit q in |0>
+    let q = alloc () in
+    let q1 = alloc () in
+    //apply H to it twice
+    apply_gate (hadamard q);
+    apply_gate (hadamard q);
+    //now we know q is in state H (H |0>)
+    assert_ (pts_to (single q) (hadamard q (hadamard q (singleton q false))));
+    //call the lemma below, and prove that q is actually back to |0>
+    hadamard_self_adjoint q;
+    rewrite (pts_to (single q) _)
+            (pts_to (single q) (singleton q false)); //use hadamard_self_adjoint to prove 
+                                                     //that q is back to its initial state
+    //discard it
+    discard q _;
+    apply_gate (hadamard q1);
+    return q1
+
+
+// returning more than one qbit
+let test3 (_:unit)
+  : STT (qbit * qbit) emp 
+        (fun qs -> pts_to (single (fst qs)) (singleton _ false) `star`
+                pts_to (single (snd qs)) (singleton _ false))
+  = //allocate a qbit q in |0>
+    let q0 = alloc () in
+    let q1 = alloc () in
+    let res = q0, q1 in
+    // This is kinda ugly, but Steel currently forces you to do this kind of rewrite
+    // and doesn't implicitly convert (pts_to (single q0) _) to (pts_to (single (fst res)) _)
+    rewrite (pts_to (single q0) _)
+            (pts_to (single (fst res)) (singleton _ false));
+    rewrite (pts_to (single q1) _)
+            (pts_to (single (snd res)) (singleton _ false));            
+    return res
+
+// returning more than one qbit after gathering them
+let test4 (_:unit)
+  : STT (qbit * qbit)
+        emp
+        (fun qs -> exists_ (fun state -> 
+                   pts_to (OrdSet.union (single (fst qs)) (single (snd qs))) state `star`
+                   pure (fst qs =!= snd qs /\
+                         state == (singleton (fst qs) false `tensor` singleton (snd qs) false))))
+  = //allocate a qbit q in |0>
+    let q0 = alloc () in
+    let q1 = alloc () in
+    let _ = gather (single q0) (single q1) #_ #_ in
+    let res = (q0, q1) in
+    rewrite (pts_to _ _)
+            (pts_to (OrdSet.union (single (fst res)) (single (snd res)))
+                    (singleton (fst res) false `tensor` singleton (snd res) false));
+    (* This is super verbose, but once F* PR  2553 is merged, this should be automated *)
+    intro_pure (fst res =!= snd res /\
+               ((singleton (fst res) false `tensor` singleton (snd res) false) ==
+                (singleton (fst res) false `tensor` singleton (snd res) false)));
+    intro_exists (singleton (fst res) false `tensor` singleton (snd res) false)
+                 (fun state -> 
+                   pts_to (OrdSet.union (single (fst res)) (single (snd res))) state `star`
+                   pure (fst res =!= snd res /\
+                         state == (singleton (fst res) false `tensor` singleton (snd res) false)));
+    return res
